LeanSAT/LRAT/Internal/LRATCheckerSound.lean
@@ -14,7 +14,7 @@ namespace Internal
 open LRAT Result Formula Clause Std Sat
 
 theorem addEmptyCaseSound [DecidableEq α] [Clause α β] [Entails α σ] [Formula α β σ] (f : σ)
-    (f_readyForRupAdd : readyForRupAdd f) (rupHints: Array Nat)
+    (f_readyForRupAdd : ReadyForRupAdd f) (rupHints: Array Nat)
     (rupAddSuccess : (Formula.performRupAdd f Clause.empty rupHints).snd = true) :
     Unsatisfiable α f := by
   let f' := (performRupAdd f empty rupHints).1
@@ -36,20 +36,20 @@ theorem addEmptyCaseSound [DecidableEq α] [Clause α β] [Entails α σ] [Formu
     empty_eq, List.any_nil] at pf
 
 theorem addRupCaseSound [DecidableEq α] [Clause α β] [Entails α σ] [Formula α β σ] (f : σ)
-    (f_readyForRupAdd : readyForRupAdd f)
-    (f_readyForRatAdd : readyForRatAdd f) (c : β) (f' : σ) (rupHints : Array Nat)
+    (f_readyForRupAdd : ReadyForRupAdd f)
+    (f_readyForRatAdd : ReadyForRatAdd f) (c : β) (f' : σ) (rupHints : Array Nat)
     (heq : performRupAdd f c rupHints = (f', true))
     (restPrf : List (Action β α)) (restPrfWellFormed : ∀ (a : Action β α), a ∈ restPrf → WellFormedAction a)
     (ih : ∀ (f : σ),
-      readyForRupAdd f → readyForRatAdd f → (∀ (a : Action β α), a ∈ restPrf → WellFormedAction a) →
+      ReadyForRupAdd f → ReadyForRatAdd f → (∀ (a : Action β α), a ∈ restPrf → WellFormedAction a) →
       lratChecker f restPrf = success → Unsatisfiable α f)
     (f'_success : lratChecker f' restPrf = success) :
     Unsatisfiable α f := by
   have f'_def := rupAdd_result f c rupHints f' f_readyForRupAdd heq
-  have f'_readyForRupAdd : readyForRupAdd f' := by
+  have f'_readyForRupAdd : ReadyForRupAdd f' := by
     rw [f'_def]
     exact insert_readyForRupAdd f c f_readyForRupAdd
-  have f'_readyForRatAdd : readyForRatAdd f' := by
+  have f'_readyForRatAdd : ReadyForRatAdd f' := by
     rw [f'_def]
     exact insert_readyForRatAdd f c f_readyForRatAdd
   specialize ih f' f'_readyForRupAdd f'_readyForRatAdd restPrfWellFormed f'_success
@@ -59,21 +59,21 @@ theorem addRupCaseSound [DecidableEq α] [Clause α β] [Entails α σ] [Formula
   exact ih p pf
 
 theorem addRatCaseSound [DecidableEq α] [Clause α β] [Entails α σ] [Formula α β σ] (f : σ)
-    (f_readyForRupAdd : readyForRupAdd f) (f_readyForRatAdd : readyForRatAdd f) (c : β)
+    (f_readyForRupAdd : ReadyForRupAdd f) (f_readyForRatAdd : ReadyForRatAdd f) (c : β)
     (pivot : Literal α) (f' : σ) (rupHints : Array Nat) (ratHints : Array (Nat × Array Nat))
     (pivot_limplies_c : Limplies α pivot c) (heq : performRatAdd f c pivot rupHints ratHints = (f', true))
     (restPrf : List (Action β α)) (restPrfWellFormed : ∀ (a : Action β α), a ∈ restPrf → WellFormedAction a)
     (ih : ∀ (f : σ),
-      readyForRupAdd f → readyForRatAdd f → (∀ (a : Action β α), a ∈ restPrf → WellFormedAction a) →
+      ReadyForRupAdd f → ReadyForRatAdd f → (∀ (a : Action β α), a ∈ restPrf → WellFormedAction a) →
       lratChecker f restPrf = success → Unsatisfiable α f)
     (f'_success : lratChecker f' restPrf = success) :
     Unsatisfiable α f := by
   rw [limplies_iff_mem] at pivot_limplies_c
   have f'_def := ratAdd_result f c pivot rupHints ratHints f' f_readyForRatAdd pivot_limplies_c heq
-  have f'_readyForRupAdd : readyForRupAdd f' := by
+  have f'_readyForRupAdd : ReadyForRupAdd f' := by
     rw [f'_def]
     exact insert_readyForRupAdd f c f_readyForRupAdd
-  have f'_readyForRatAdd : readyForRatAdd f' := by
+  have f'_readyForRatAdd : ReadyForRatAdd f' := by
     rw [f'_def]
     exact insert_readyForRatAdd f c f_readyForRatAdd
   specialize ih f' f'_readyForRupAdd f'_readyForRatAdd restPrfWellFormed f'_success
@@ -84,21 +84,21 @@ theorem addRatCaseSound [DecidableEq α] [Clause α β] [Entails α σ] [Formula
   exact ih p pf
 
 theorem delCaseSound [DecidableEq α] [Clause α β] [Entails α σ] [Formula α β σ] (f : σ)
-    (f_readyForRupAdd : readyForRupAdd f) (f_readyForRatAdd : readyForRatAdd f) (ids : Array Nat)
+    (f_readyForRupAdd : ReadyForRupAdd f) (f_readyForRatAdd : ReadyForRatAdd f) (ids : Array Nat)
     (restPrf : List (Action β α))
     (restPrfWellFormed : ∀ (a : Action β α), a ∈ restPrf → WellFormedAction a)
     (ih : ∀ (f : σ),
-      readyForRupAdd f → readyForRatAdd f → (∀ (a : Action β α), a ∈ restPrf → WellFormedAction a) →
+      ReadyForRupAdd f → ReadyForRatAdd f → (∀ (a : Action β α), a ∈ restPrf → WellFormedAction a) →
       lratChecker f restPrf = success → Unsatisfiable α f)
     (h : lratChecker (Formula.delete f ids) restPrf = success) :
     Unsatisfiable α f := by
   intro p pf
-  have f_del_readyForRupAdd : readyForRupAdd (Formula.delete f ids) := delete_readyForRupAdd f ids f_readyForRupAdd
-  have f_del_readyForRatAdd : readyForRatAdd (Formula.delete f ids) := delete_readyForRatAdd f ids f_readyForRatAdd
+  have f_del_readyForRupAdd : ReadyForRupAdd (Formula.delete f ids) := delete_readyForRupAdd f ids f_readyForRupAdd
+  have f_del_readyForRatAdd : ReadyForRatAdd (Formula.delete f ids) := delete_readyForRatAdd f ids f_readyForRatAdd
   exact ih (delete f ids) f_del_readyForRupAdd f_del_readyForRatAdd restPrfWellFormed h p (limplies_delete p pf)
 
 theorem lratCheckerSound [DecidableEq α] [Clause α β] [Entails α σ] [Formula α β σ] (f : σ)
-    (f_readyForRupAdd : readyForRupAdd f) (f_readyForRatAdd : readyForRatAdd f)
+    (f_readyForRupAdd : ReadyForRupAdd f) (f_readyForRatAdd : ReadyForRatAdd f)
     (prf : List (Action β α)) (prfWellFormed : ∀ a : Action β α, a ∈ prf → WellFormedAction a) :
     lratChecker f prf = success → Unsatisfiable α f := by
   induction prf generalizing f
